Main.lean
@@ -16,19 +16,19 @@ open Batteries (AssocList)
 open Graphiti
 
 structure CmdArgs where
-  outputFile : Option System.FilePath
-  inputFile : Option System.FilePath
-  logFile : Option System.FilePath
-  logStdout : Bool
-  noDynamaticDot : Bool
-  parseOnly : Bool
-  graphitiOracle : Option String
-  slow : Bool
-  reverse : Bool
-  help : Bool
+  outputFile : Option System.FilePath := none
+  inputFile : Option System.FilePath := none
+  logFile : Option System.FilePath := none
+  logStdout : Bool := false
+  noDynamaticDot : Bool := false
+  parseOnly : Bool := false
+  graphitiOracle : String := "graphiti_oracle"
+  slow : Bool := false
+  reverse : Bool := false
+  help : Bool := false
 deriving Inhabited
 
-def CmdArgs.empty : CmdArgs := default
+def CmdArgs.empty : CmdArgs := {}
 
 /--
 Split short options up into multiple options: i.e. '-ol' will become '-o -l'.
@@ -93,9 +93,9 @@ def reduceSink := [SplitSinkRight.rewrite, SplitSinkLeft.rewrite, PureSink.rewri
 def movePureJoin := [PureJoinLeft.rewrite, PureJoinRight.rewrite, PureSplitRight.rewrite, PureSplitLeft.rewrite]
 
 def normaliseLoop (e : ExprHigh String) : RewriteResult (ExprHigh String) := do
-  let rw ← rewrite_fix (pref := "rw_loop0") e forkRewrites
-  let rw ← rewrite_loop (pref := "rw_loop1") rw combineRewrites
-  let rw ← rewrite_fix (pref := "rw_loop2") rw reduceRewrites
+  let rw ← rewrite_fix e forkRewrites
+  let rw ← rewrite_loop rw combineRewrites
+  let rw ← rewrite_fix rw reduceRewrites
   return rw
 
 def allPattern (f : String → Bool) : Pattern String :=
@@ -104,46 +104,47 @@ def allPattern (f : String → Bool) : Pattern String :=
 def pureGeneration (rw : ExprHigh String) (p1 p2 : Pattern String) : RewriteResult (ExprHigh String) := do
   -- Convert most of the dataflow graph to pure.
   -- let rw ← rewrite_fix rw <| PureRewrites.specialisedPureRewrites LoopRewrite.nonPureMatcher
-  let rw ← rewrite_fix (pref := "rw_pure1") rw <| PureRewrites.specialisedPureRewrites <| p1
+  let rw ← rewrite_fix rw <| PureRewrites.specialisedPureRewrites <| p1
   -- Move forks as high as possible, and also move pure over joins and under sinks.  Also remove sinks.
-  let rw ← rewrite_fix (pref := "rw_pure2") rw <| [ForkPure.rewrite, ForkJoin.rewrite] ++ movePureJoin ++ reduceSink
+  let rw ← rewrite_fix rw <| [ForkPure.rewrite, ForkJoin.rewrite] ++ movePureJoin ++ reduceSink
   -- Turn forks into pure.
-  let rw ← rewrite_fix (pref := "rw_pure3") rw <| PureRewrites.specialisedPureRewrites p2
+  let rw ← rewrite_fix rw <| PureRewrites.specialisedPureRewrites p2
   -- Move pures to the top and bottom again, we are left with split and join nodes.
-  let rw ← rewrite_fix (pref := "rw_pure4") rw <| [PureSeqComp.rewrite] ++ movePureJoin ++ reduceSink
+  let rw ← rewrite_fix rw <| [PureSeqComp.rewrite] ++ movePureJoin ++ reduceSink
   return rw
 
 def pureGenerator' (n : Nat) (g : ExprHigh String) : List JSLangRewrite → Nat → RewriteResult (ExprHigh String)
 | _, 0 => throw <| .error "No fuel"
 | [], fuel+1 => pure g
 | [jsRw], fuel+1 => do
-  let rw ← jsRw.mapToRewrite.run s!"jsrw_{n}_{fuel}" g
-  let rw ← rewrite_fix (pref := s!"jsrw3_{n}_{fuel}") rw ([PureSeqComp.rewrite] ++ movePureJoin ++ reduceSink)
+  let rw ← jsRw.mapToRewrite.run g
+  let rw ← rewrite_fix rw ([PureSeqComp.rewrite] ++ movePureJoin ++ reduceSink)
   return rw
 | jsRw :: rst, fuel+1 => do
   -- addRewriteInfo {(default : RewriteInfo) with debug := .some s!"{repr jsRw}"}
-  let rw ← jsRw.mapToRewrite.run s!"jsrwR_{n}_{fuel}" g
+  let rw ← jsRw.mapToRewrite.run g
   let rst ← update_state JSLang.upd rst
 
-  let (rw, rst) ← rewrite_fix_rename (pref := s!"jsrw2_{n}_{fuel}") rw ([PureSeqComp.rewrite] ++ movePureJoin ++ reduceSink) JSLang.upd rst
+  let (rw, rst) ← rewrite_fix_rename rw ([PureSeqComp.rewrite] ++ movePureJoin ++ reduceSink) JSLang.upd rst
   pureGenerator' n rw rst fuel
 
 def pureGenerator n g js := pureGenerator' n g js (js.length + 1)
 
-def eggPureGenerator (fuel : Nat) (parsed : CmdArgs) (p : Pattern String) (g : ExprHigh String) (st : List RewriteInfo) : IO (ExprHigh String × List RewriteInfo) := do
+def eggPureGenerator (fuel : Nat) (parsed : CmdArgs) (p : Pattern String) (g : ExprHigh String) (st : RewriteState)
+  : IO (ExprHigh String × RewriteState) := do
   match fuel with
   | 0 => throw <| .userError s!"{decl_name%}: no fuel"
   | fuel+1 =>
-    let jsRw ← rewriteWithEgg (eggCmd := parsed.graphitiOracle.getD "graphiti_oracle") p g
+    let jsRw ← rewriteWithEgg (eggCmd := parsed.graphitiOracle) p g
     if jsRw.length = 0 then return (g, st)
     IO.eprintln (repr jsRw)
     match pureGenerator fuel g jsRw |>.run st with
     | .ok g' st' => eggPureGenerator fuel parsed p g' st'
     | .error e st' =>
       match parsed.logFile with
-      | .some lfile => IO.FS.writeFile lfile <| toString <| Lean.toJson st'
+      | .some lfile => IO.FS.writeFile lfile <| toString <| Lean.toJson st'.1
       | .none =>
-        if parsed.logStdout then IO.println <| Lean.toJson st'
+        if parsed.logStdout then IO.println <| Lean.toJson st'.1
       IO.eprintln e
       IO.Process.exit 1
 
@@ -156,13 +157,13 @@ def renameAssoc (g : ExprHigh String) (assoc : AssocList String (AssocList Strin
 
 def renameAssocAll assoc (rlist : List RewriteInfo) (g : ExprHigh String) := rlist.foldl (renameAssoc g) assoc
 
-def writeLogFile (parsed : CmdArgs) (st : List RewriteInfo) := do
+def writeLogFile (parsed : CmdArgs) (st : RewriteState) := do
   match parsed.logFile with
-  | .some lfile => IO.FS.writeFile lfile <| toString <| Lean.toJson st
+  | .some lfile => IO.FS.writeFile lfile <| toString <| Lean.toJson st.1
   | .none =>
-    if parsed.logStdout then IO.println <| Lean.toJson st
+    if parsed.logStdout then IO.println <| Lean.toJson st.1
 
-def runRewriter {α} (parsed : CmdArgs) (g : α) (st : List RewriteInfo) (r : RewriteResult α) : IO (α × List RewriteInfo) :=
+def runRewriter {α} (parsed : CmdArgs) (g : α) (st : RewriteState) (r : RewriteResult α) : IO (α × RewriteState) :=
   match r.run st with
   | .ok a st' => writeLogFile parsed st' *> pure (a, st')
   | .error .done st' => writeLogFile parsed st' *> pure (g, st')
@@ -171,7 +172,7 @@ def runRewriter {α} (parsed : CmdArgs) (g : α) (st : List RewriteInfo) (r : Re
     writeLogFile parsed st'
     IO.Process.exit 1
 
-def runRewriter' {α} (parsed : CmdArgs) (st : List RewriteInfo) (r : RewriteResult α) : IO (α × List RewriteInfo) :=
+def runRewriter' {α} (parsed : CmdArgs) (st : RewriteState) (r : RewriteResult α) : IO (α × RewriteState) :=
   match r.run st with
   | .ok a st' => writeLogFile parsed st' *> pure (a, st')
   | .error p st' => do
@@ -179,20 +180,20 @@ def runRewriter' {α} (parsed : CmdArgs) (st : List RewriteInfo) (r : RewriteRes
     writeLogFile parsed st'
     IO.Process.exit 1
 
-def rewriteGraph (parsed : CmdArgs) (g : ExprHigh String) (st : List RewriteInfo)
-    : IO (ExprHigh String × List RewriteInfo × List RewriteInfo) := do
+def rewriteGraph (parsed : CmdArgs) (g : ExprHigh String) (st : RewriteState)
+    : IO (ExprHigh String × RewriteState × RewriteState) := do
   let (rewrittenExprHigh, st) ← runRewriter parsed g st (normaliseLoop g)
   let (rewrittenExprHigh, st) ← runRewriter parsed rewrittenExprHigh st (pureGeneration rewrittenExprHigh LoopRewrite.nonPureMatcher LoopRewrite.nonPureForkMatcher)
   let (rewrittenExprHigh, st) ← eggPureGenerator 100 parsed LoopRewrite.boxLoopBodyOther rewrittenExprHigh st <* writeLogFile parsed st
-  let (rewrittenExprHigh, st) ← runRewriter parsed rewrittenExprHigh st (LoopRewrite2.rewrite.run "loop_rw_" rewrittenExprHigh)
+  let (rewrittenExprHigh, st) ← runRewriter parsed rewrittenExprHigh st (LoopRewrite2.rewrite.run rewrittenExprHigh)
   return (rewrittenExprHigh, st, st)
 
-def rewriteGraphAbs (parsed : CmdArgs) (g : ExprHigh String) (st : List RewriteInfo)
-    : IO (ExprHigh String × List RewriteInfo × List RewriteInfo) := do
+def rewriteGraphAbs (parsed : CmdArgs) (g : ExprHigh String) (st : RewriteState)
+    : IO (ExprHigh String × RewriteState × RewriteState) := do
   let (g, st) ← runRewriter parsed g st (normaliseLoop g)
 
   let a : Abstraction String := ⟨λ g => LoopRewrite.boxLoopBody g >>= λ (a, _b) => pure (a, []), "M"⟩
-  let ((bigg, concr), st) ← runRewriter' parsed st <| a.run "abstr_" g
+  let ((bigg, concr), st) ← runRewriter' parsed st <| a.run g
   let .some g := concr.expr.higherSS | throw <| .userError s!"{decl_name%}: failed to higher expr"
   -- IO.print <| bigg
   let st_final := st
@@ -205,12 +206,12 @@ def rewriteGraphAbs (parsed : CmdArgs) (g : ExprHigh String) (st : List RewriteI
 
   -- The first concretisation replaces "M" by the "pure" block
   let newConcr : Concretisation String := ⟨subexpr, concr.2⟩
-  let (g, st) ← runRewriter' parsed st <| newConcr.run "concr_" bigg
+  let (g, st) ← runRewriter' parsed st <| newConcr.run bigg
 
-  let (g, st) ← runRewriter parsed g st (LoopRewrite2.rewrite.run "loop_rw_" g)
+  let (g, st) ← runRewriter parsed g st (LoopRewrite2.rewrite.run g)
 
   let newConcr' : Concretisation String := ⟨concr.1, typ⟩
-  let (g, st) ← runRewriter parsed g st <| newConcr'.run "concr2_" g
+  let (g, st) ← runRewriter parsed g st <| newConcr'.run g
 
   return (g, st_final, st)
 
@@ -248,13 +249,13 @@ def reverse_rewrite_with_index (rinfo : RewriteInfo) : RewriteResult (Rewrite St
     | _ => rewrite_index.find? name
   reverse_rewrite rw rinfo
 
-def reverseRewrites (parsed : CmdArgs) (g : ExprHigh String) (st : List RewriteInfo)
-    : IO (ExprHigh String × List RewriteInfo) := do
-  let st_worklist := st.reverse.tail.take 158
+def reverseRewrites (parsed : CmdArgs) (g : ExprHigh String) (st : RewriteState)
+    : IO (ExprHigh String × RewriteState) := do
+  let st_worklist := st.1.reverse.tail.take 158
 
   let (g, st) ← runRewriter' parsed st <| st_worklist.foldlM (λ g rinfo => do
       let rewrite ← reverse_rewrite_with_index rinfo
-      rewrite.run' (norm := false) "reverse" g
+      rewrite.run' (norm := false) g
     ) g
 
   return (g, st)
@@ -277,7 +278,7 @@ def main (args : List String) : IO Unit := do
   let (exprHigh, assoc) ← IO.ofExcept fileContents.toExprHigh
 
   let mut rewrittenExprHigh := exprHigh
-  let mut st : List RewriteInfo := default
+  let mut st : RewriteState := default
 
   if !parsed.parseOnly then
     let (g', _, st') ← (if parsed.slow then rewriteGraph else rewriteGraphAbs) parsed rewrittenExprHigh st
@@ -286,7 +287,7 @@ def main (args : List String) : IO Unit := do
   -- IO.println (repr (rewrittenExprHigh.modules.toList.map Prod.fst))
   let some l :=
     if parsed.noDynamaticDot then pure (toString rewrittenExprHigh)
-    else dynamaticString rewrittenExprHigh (renameAssocAll assoc st rewrittenExprHigh)
+    else dynamaticString rewrittenExprHigh (renameAssocAll assoc st.1 rewrittenExprHigh)
     | IO.eprintln s!"Failed to print ExprHigh: {rewrittenExprHigh}"
   -- IO.print (repr rewrittenExprHigh)
 
